\documentclass[fleqn]{report}

\input{C:/Users/Paul Taveneaux/Desktop/document/progra/latex/files/preamble_dark}
\input{C:/Users/Paul Taveneaux/Desktop/document/progra/latex/files/macros}
\input{C:/Users/Paul Taveneaux/Desktop/document/progra/latex/files/letterfonts}

\title{formulas used by Pi-chuck}
\author{Paul TAVENEAUX}
\date{\today}

\pagecolor{black}
\color{white}

\begin{document}
\maketitle
\newpage

\section{Original formula}
\[
  \frac{1}{\pi} = \frac{1}{426880\sqrt{10005}}\sum_{ k = 0 }^{\infty}\frac{(-1)^k(6k)!(13591409 + 545140134k)}{(3k)!(k!)^3640320^{3k}}
\]

\section{$\pi$ in terms of $a$ and $b$}

\begin{align*}
  \frac{1}{\pi} &= \frac{1}{426880\sqrt{10005}}\left[13591409\sum_{k = 0}^{\infty}\frac{(-1)^k(6k)!}{(3k)!(k!)^3640320^{3k}} + 545140134\sum_{k = 0}^{\infty}\frac{(-1)^k(6k)!k}{(3k)!(k!)^3640320^{3k}}\right]\\
  \pi &= \frac{426880\sqrt{10005}}{1359140a + 545140134b}\\
\end{align*}
with
\begin{align*}
  a &= \sum_{k = 0}^{\infty}\frac{(-1)^k(6k)!}{(3k)!(k!)^3640320^{3k}}\\
  \text{and} \quad b &= \sum_{k = 0}^{\infty}\frac{(-1)^k(6k)!k}{(3k)!(k!)^3640320^{3k}}
\end{align*}

\section{$\pi$ in terms of $a_k$ and $b_k$}
let $(a_n)_{n \in \N}$ be a series such that:
\[
  \forall n \in \N, a_n = \frac{(-1)^k(6k)!k}{(3k)!(k!)^3640320^{3k}}
.\]
it then follows that :
\[
a = \sum_{k=0}^{\infty} a_k
.\] 

\noindent
let $(b_n)_{n \in \N}$ be a series defined by:
\[
\forall n  \in \N,\ b_n = n * a_n
.\] 
It then follows that:
\[
  b = \sum_{k=0}^{\infty} b_k
.\] 

\section{recursive definition of the $a_n$s and $b_n$s}

\begin{align*}
  \left\{
    \begin{aligned}
    a_0 &= 
    \end{aligned}
  \right.
\end{align*}

\end{document}
